Lending Protocol - Dafny

dafny/src/lendingProtocol.dfy
@@ -15,54 +15,88 @@ class LendingProtocol {
     var totalBorrow: u256
     var totalReserve: u256
     var totalDeposit: u256
-    var maxLTV: u256
+    const maxLTV: u256 := 4
     var ethTreasury: u256
     var totalCollateral: u256
-    var baseRate: u256
-    var fixedAnnuBorrowRate: u256
+    const baseRate: u256 := 20000000000000000
+    const fixedAnnuBorrowRate: u256 := 300000000000000000
 
     var usersCollateral: mapping<u160, u256>
     var usersBorrowed: mapping<u160, u256>
 
-    var WAD: u256
+    const WAD: u256 := 1000000000000000000
 
     constructor() {
-        maxLTV := 4;
-        baseRate := 20000000000000000;
-        fixedAnnuBorrowRate := 300000000000000000;
-
-        WAD := 1000000000000000000;
+        totalDeposit := 1000;
+        totalBorrow := 20;
 
         usersCollateral := Map(map[], 0);
         usersBorrowed := Map(map[], 0);
     }
 
     method utilizationRatio() returns (utilizationRatio: u256)
-    ensures utilizationRatio == this.totalBorrow / this.totalDeposit
+    // ensures utilizationRatio == this.totalBorrow / this.totalDeposit
+    requires this.fixedAnnuBorrowRate > this.baseRate
+    requires this.totalBorrow as nat * (this.fixedAnnuBorrowRate - this.baseRate) as nat <= MAX_U256 as nat
+    requires this.totalDeposit != 0
     {
-        utilizationRatio := Fixed.Div(this.totalBorrow, this.totalDeposit);
+        // var num: u256 := Sub(this.fixedAnnuBorrowRate, this.baseRate);
+        // var mul: u256 := Mul(this.totalBorrow, num);
+        // utilizationRatio := Fixed.Div(mul, this.totalDeposit);
+
+        var num: u256 := this.fixedAnnuBorrowRate - this.baseRate;
+        var mul: u256 := this.totalBorrow * num;
+        utilizationRatio := mul / this.totalDeposit;
     }
 
-    method interestMultiplier() returns (interestMultiplier: u256)
+    method interestMultiplier() returns (interestMul: u256)
+    requires this.fixedAnnuBorrowRate > this.baseRate
+    requires this.totalBorrow as nat * (this.fixedAnnuBorrowRate - this.baseRate) as nat <= MAX_U256 as nat
+    requires this.totalDeposit != 0
     {
         var uRatio: u256 := utilizationRatio();
-        var num: u256 := Sub(this.fixedAnnuBorrowRate, this.baseRate);
-        interestMultiplier := Fixed.Div(num, uRatio);
+        var num: u256 := this.fixedAnnuBorrowRate - this.baseRate;
+        if uRatio == 0 {
+            interestMul := 0;
+        }
+        else {
+            interestMul := num / uRatio;
+        }
     }
     
 
     method borrowRate() returns (rate: u256)
-    requires rate > 0 {
+    requires this.fixedAnnuBorrowRate > this.baseRate
+    requires this.totalBorrow as nat * (this.fixedAnnuBorrowRate - this.baseRate) as nat <= MAX_U256 as nat
+    requires this.totalDeposit != 0
+    ensures rate as nat <= MAX_U256 as nat
+    {
         var uRatio: u256 := utilizationRatio();
-
+        var interestMul: u256 := interestMultiplier();
+        var product:u256 :=0;
+        if uRatio as nat * interestMul as nat <= MAX_U256 as nat {
+            product := uRatio * interestMul;
+        }
+        rate := 0;
+        if product as nat + baseRate as nat <= MAX_U256 as nat {
+            rate := product + baseRate;
+        }
     }
 
-
     method calculateBorrowFee(amount: u256) returns (fee: u256, paid: u256)
-    requires amount > 0
-
+    requires this.fixedAnnuBorrowRate > this.baseRate
+    requires this.totalBorrow as nat * (this.fixedAnnuBorrowRate - this.baseRate) as nat <= MAX_U256 as nat
+    requires this.totalDeposit != 0
     {
-        totalDeposit := totalDeposit;
-        return Ok(());
+        var borrowRate: u256 := borrowRate();
+        fee := 0;
+        if amount as nat * borrowRate as nat <= MAX_U256 as nat {
+            // fee := amount * borrowRate;
+            fee := Mul(amount, borrowRate);
+        }
+        paid := 0;
+        if amount as nat - fee as nat > 0 as nat {
+            paid := amount - fee;
+        }
     }
 }
